Db/Migration/Main.lean
@@ -1,0 +1,5 @@
+import Db.Migration.Recipe
+
+-- TODO: make this a proper CLI
+def main : IO Unit := do
+  IO.println "Generating migrations."
